Partial fix for append_left proof

pulse/examples/steel/Selectors.Tree.fst
@@ -6,27 +6,23 @@ open Steel.SelEffect
 
 module Spec = FStar.Trees
 
-#set-options "--fuel 4 --ifuel 2 --z3rlimit 30"
+#set-options "--fuel 1 --ifuel 1 --z3rlimit 30"
 
 let rec append_left #a ptr v =
-  if is_null_t ptr then begin
+  if is_null_t ptr then (
     drop_linked_tree_leaf ptr;
     let node = mk_node v null_t null_t in
     let new_tree = alloc node in
     intro_linked_tree_leaf #a ();
     intro_linked_tree_leaf #a ();
-    admit();
+    assume(not(is_null_t new_tree));
     pack_tree new_tree null_t null_t;
-    admit();
-    noop ();
     new_tree
-  end else begin
+  ) else (
     let node = unpack_tree ptr in
     let new_left = append_left (get_left node) v in
     let new_node = mk_node (get_data node) new_left (get_right node) in
     write ptr new_node;
     pack_tree ptr new_left (get_right node);
-    admit();
-    noop ();
     ptr
-  end
+  )
